in progress: module system

templates/hindsight/hindsight.v
@@ -7,12 +7,11 @@ From iris.proofmode Require Import tactics.
 From iris.heap_lang Require Import proofmode par.
 From iris.heap_lang.lib Require Import nondet_bool.
 From iris.bi.lib Require Import fractional.
-From diaframe.heap_lang Require Import proof_automation atomic_specs wp_auto_lob.
 Require Export one_shot_proph typed_proph.
 Require Export multiset_flows keyset_ra.
 
 
-Module Type ABSTRACT_DATA_TYPE.
+Module Type DATA_STRUCTURE.
   
   Parameter dsOp : val.
   Parameter Op : Type.
@@ -26,7 +25,8 @@ Module Type ABSTRACT_DATA_TYPE.
   Coercion resT_to_base_lit : resT >-> base_lit.
   Parameter resT_from_val : val -> option resT.
   Parameter resT_to_val : resT -> val.
-  Parameter resT_inj_prop : ∀ (r : resT), resT_from_val (resT_to_val r) = Some r.
+  Parameter resT_inj_prop : 
+    ∀ (r : resT), resT_from_val (resT_to_val r) = Some r.
   Definition resTProph : TypedProphSpec :=
     mkTypedProphSpec resT resT_from_val resT_to_val resT_inj_prop.
   Definition resTTypedProph `{!heapGS Σ} := make_TypedProph resTProph.
@@ -35,16 +35,12 @@ Module Type ABSTRACT_DATA_TYPE.
   Parameter seq_spec : Op -> absT -> absT -> resT -> Prop.
   Parameter seq_spec_dec : ∀ op c c' res, Decision (seq_spec op c c' res).
   Parameter updater_thread: Op -> resT -> bool.
-  Parameter updater_thread_dec: ∀ op res b, Decision (updater_thread op res = b).
+  Parameter updater_thread_dec: 
+    ∀ op res b, Decision (updater_thread op res = b).
 
   Parameter Op_inhabited : Inhabited Op.
   Parameter absTUR_discrete : CmraDiscrete absTUR.
   Parameter resT_inhabited : Inhabited resT.
-
-End ABSTRACT_DATA_TYPE.
-
-Module Type DATA_STRUCTURE (ADT: ABSTRACT_DATA_TYPE).
-  Import ADT.
 
   Parameter snapshotUR : ucmra.
   Definition snapshot := ucmra_car snapshotUR.
@@ -55,12 +51,21 @@ Module Type DATA_STRUCTURE (ADT: ABSTRACT_DATA_TYPE).
   
   Parameter snapshot_leibnizequiv : LeibnizEquiv (snapshot).
   Parameter snapshot_inhabited : Inhabited snapshot.
+  
+(*   Parameter dsG : gFunctors -> Set. *)
+  (* Parameter dsΣ : gFunctors. *)
+  
+  (* Parameter subG_dsΣ : ∀ Σ, subG dsΣ Σ → dsG Σ. *)
+  
+  Context `{!heapGS Σ, !dsG Σ}.
+  
+  Parameter ds_inv : gmap nat snapshot -> nat -> snapshot -> iProp Σ.
 
 End DATA_STRUCTURE.  
 
 
-Module HINDSIGHT_DEFS (ADT: ABSTRACT_DATA_TYPE) (DS : DATA_STRUCTURE ADT).
-  Import ADT DS.
+Module HINDSIGHT_DEFS (DS : DATA_STRUCTURE).
+  Import DS.
   
   Global Instance snapshotUR_discrete' : CmraDiscrete snapshotUR.
   Proof.
@@ -107,29 +112,29 @@ Module HINDSIGHT_DEFS (ADT: ABSTRACT_DATA_TYPE) (DS : DATA_STRUCTURE ADT).
                               gmapUR proph_id $ 
                                 agreeR $ prodO natO gnameO.
 
-  Class dsG Σ := DS {
-                  dsG_auth_natG :> inG Σ auth_natUR;
-                  dsG_agree_snapshotG :> inG Σ agree_snapshotR;
-                  dsG_frac_absTG :> inG Σ frac_absTR;
-                  dsG_historyG :> inG Σ historyR;
-                  dsG_auth_historyG :> inG Σ auth_historyR;
-                  dsG_tokenG :> inG Σ tokenUR;
-                  dsG_frac_historyG :> inG Σ frac_historyR;
-                  dsG_set_tidG :> inG Σ set_tidR;
-                  dsG_thread_viewG :> inG Σ thread_viewR
+  Class hsG Σ := HS {
+                  hsG_auth_natG :> inG Σ auth_natUR;
+                  hsG_agree_snapshotG :> inG Σ agree_snapshotR;
+                  hsG_frac_absTG :> inG Σ frac_absTR;
+                  hsG_historyG :> inG Σ historyR;
+                  hsG_auth_historyG :> inG Σ auth_historyR;
+                  hsG_tokenG :> inG Σ tokenUR;
+                  hsG_frac_historyG :> inG Σ frac_historyR;
+                  hsG_set_tidG :> inG Σ set_tidR;
+                  hsG_thread_viewG :> inG Σ thread_viewR
                  }.
                  
-  Definition dsΣ : gFunctors :=
+  Definition hsΣ : gFunctors :=
     #[ GFunctor auth_natUR; GFunctor agree_snapshotR;
        GFunctor frac_absTR; GFunctor historyR;
        GFunctor auth_historyR; GFunctor tokenUR; 
        GFunctor frac_historyR; GFunctor set_tidR;
        GFunctor thread_viewR ].
   
-  Global Instance subG_dsΣ {Σ} : subG dsΣ Σ → dsG Σ.
+  Global Instance subG_hsΣ {Σ} : subG hsΣ Σ → hsG Σ.
   Proof. solve_inG. Qed.
-
-  Context {Σ} `{!heapGS Σ, !dsG Σ}.
+  
+  Context `{!heapGS Σ, !hsG Σ}.
   Notation iProp := (iProp Σ).
   Implicit Types M : gmap nat snapshot.
   Implicit Types T : nat.
@@ -210,20 +215,14 @@ Module HINDSIGHT_DEFS (ADT: ABSTRACT_DATA_TYPE) (DS : DATA_STRUCTURE ADT).
       ∗ own γ_ght (● hγt) ∗ ⌜dom hγt = R⌝  
       ∗ ([∗ set] t_id ∈ R, Reg N γ_t γ_s γ_ght t_id M).
   
-  Definition ds_inv N γ_t γ_s γ_m γ_td γ_ght template_inv : iProp :=
+  Definition main_inv N γ_t γ_s γ_m γ_td γ_ght : iProp :=
     inv (cntrN N)
     (∃ M T (s: snapshot),
-      dsRepI γ_s (abs s) ∗ ⌜abs (M !!! T) = abs s⌝
+      dsRepI γ_s (abs s) ∗ ⌜M !!! T ≡ s⌝
     ∗ hist γ_t γ_m M T
     ∗ helping_inv N γ_t γ_s γ_td γ_ght M
-    ∗ template_inv M T s).
-(*    
-  Instance dsRep_timeless : ∀ γ_s C, Timeless (dsRep γ_s C).
-  Proof.
-    intros γ_s C. rewrite /dsRep. Search Timeless. 
-    apply own_timeless; apply _.
-  Qed.   
-*)    
+    ∗ ds_inv M T s).
+
   Definition update_helping_protocol N γ_t γ_s γ_td γ_ght : iProp :=
         ∀ M T n s, 
           ⌜map_max M = T⌝ -∗   
@@ -234,647 +233,4 @@ Module HINDSIGHT_DEFS (ADT: ABSTRACT_DATA_TYPE) (DS : DATA_STRUCTURE ADT).
     
 End HINDSIGHT_DEFS.
 
-Module Type HINDSIGHT_SPEC (ADT: ABSTRACT_DATA_TYPE) (DS : DATA_STRUCTURE ADT).
-  Module DEFS := HINDSIGHT_DEFS ADT DS.
-  Import ADT DS DEFS.
 
-  Parameter dsOp_spec: ∀ N γ_s γ_t γ_m γ_td γ_ght op (r: Node) template_inv γ_sy t_id t0,
-          ds_inv N γ_t γ_s γ_m γ_td γ_ght template_inv -∗
-            □ update_helping_protocol N γ_t γ_s γ_td γ_ght -∗
-              thread_vars γ_t γ_ght γ_sy t_id t0 -∗
-                {{{ True }}} 
-                     dsOp (Op_to_val op) #r
-                {{{ res, RET #res; past_lin_witness γ_m op res t0  }}}.
-
-End HINDSIGHT_SPEC.
-
-Module CLIENT_SPEC (ADT: ABSTRACT_DATA_TYPE) (DS : DATA_STRUCTURE ADT) 
-  (HS: HINDSIGHT_SPEC ADT DS).
-  (* Module DEFS := HINDSIGHT_DEFS ADT DS. *)
-  Import ADT DS HS DEFS.
-
-  Definition dsOp' : val :=
-    λ: "OP" "r",     
-      let: "t_id" := NewProph in
-      let: "p" := NewProph in
-      let: "v" := dsOp "OP" "r" in
-      resolve_proph: "p" to: "v";;
-      "v".
-        
-  (** Proofs *)
-
-  Lemma dsOp'_spec N γ_s γ_t γ_m γ_td γ_ght template_inv op r :
-          ds_inv N γ_t γ_s γ_m γ_td γ_ght template_inv -∗
-              <<< ∀∀ a, dsRep γ_s a >>> 
-                     dsOp' (Op_to_val op) #r @ ↑(cntrN N)
-              <<< ∃∃ a' res, dsRep γ_s a' ∗ ⌜seq_spec op a a' res⌝, RET #res >>>.
-  Proof.
-(*  
-    iIntros "#HInv" (Φ) "AU". wp_lam. 
-    wp_pure credit:"Hc". wp_pures.
-    wp_apply wp_new_proph1; try done.
-    iIntros (tid vtid)"Htid". wp_pures.
-    wp_apply (typed_proph_wp_new_proph1 resTTypedProph); first done.
-    iIntros (vp p)"Hproph". wp_pures.
-    iApply fupd_wp.
-    iInv "HInv" as (M0 T0 s0) "(>HCntr & >%Habs0 & >Hist & Help & Templ)". 
-    iDestruct "Help" as (R hγt)"(>HR & >Hγt 
-                                & >Domm_hγt & Hstar_reg)".
-    iAssert (▷ (⌜tid ∉ R⌝ 
-            ∗ ([∗ set] t_id ∈ R, Reg N γ_t γ_s γ_ght t_id M0) 
-            ∗ proph1 tid vtid))%I with "[Hstar_reg Htid]" 
-            as "(>% & Hstar_reg & Htid)".
-    { destruct (decide (tid ∈ R)); try done.
-      - iEval (rewrite (big_sepS_elem_of_acc _ (R) tid); 
-                            last by eauto) in "Hstar_reg".
-        iDestruct "Hstar_reg" as "(Hreg & Hstar_reg')".
-        iDestruct "Hreg" as (? ? ? ? ? ? ?)"(H' & _)".
-        iAssert (▷ False)%I with "[H' Htid]" as "HF".
-        iApply (proph1_exclusive tid with "[Htid]"); try done.
-        iNext. iExFalso; try done.
-      - iNext. iFrame. by iPureIntro. }
-    rename H into tid_notin_R.
-    
-    iMod (own_update γ_td (● R) (● (R ∪ {[tid]})) with "[$HR]") as "HR".
-    { apply (auth_update_auth _ _ (R ∪ {[tid]})).
-      apply gset_local_update. set_solver. }
-    iMod (own_update γ_td (● (R ∪ {[tid]})) (● (R ∪ {[tid]}) ⋅ ◯ {[tid]}) 
-              with "[$HR]") as "(HR & #FP_t)".
-    { apply (auth_update_dfrac_alloc _ (R ∪ {[tid]}) ({[tid]})).
-      apply gset_included. clear; set_solver. }
-    
-    iMod (own_alloc (to_frac_agree (1) (M0))) 
-            as (γ_sy)"Hfr_t". { try done. }        
-    iEval (rewrite <-Qp.half_half) in "Hfr_t".      
-    iEval (rewrite (frac_agree_op (1/2) (1/2) _)) in "Hfr_t". 
-    iDestruct "Hfr_t" as "(Hreg_sy1 & Hreg_sy2)".  
-    
-    iDestruct "Domm_hγt" as %Domm_hγt.
-    set (<[ tid := to_agree (T0, γ_sy) ]> hγt) as hγt'.
-    iDestruct (own_update _ _ 
-      (● hγt' ⋅ ◯ {[ tid := to_agree (T0, γ_sy) ]})
-             with "Hγt") as ">Hγt".
-    { apply auth_update_alloc. 
-      rewrite /hγt'.
-      apply alloc_local_update; last done.
-      rewrite <-Domm_hγt in tid_notin_R.
-      by rewrite not_elem_of_dom in tid_notin_R. }
-    iDestruct "Hγt" as "(Hγt & #Hreg_gh)".
-  
-    iMod (own_alloc (Excl ())) as (γ_tk) "Token"; first try done.
-  
-    assert (map_max M0 = T0) as M_max. { admit. }
-    iAssert (own γ_t (◯ (MaxNat T0))) as "HfragT0".
-    { admit. }
-    
-    assert (∀ op c c' res, Decision (¬ seq_spec op c c' res)) as neg_seq_spec_dec.
-    { intros; apply not_dec. apply seq_spec_dec. }
-    assert (∀ op c res, Decision (updater_thread op res = true 
-              ∨ (updater_thread op res = false 
-                  ∧ ¬ seq_spec op c c res))) as Hdec.
-    { intros. apply or_dec; try apply updater_thread_dec.
-      apply and_dec; try apply updater_thread_dec.
-      apply neg_seq_spec_dec. }
-      
-    destruct (decide (updater_thread op vp = true 
-      ∨ (updater_thread op vp = false 
-          ∧ ¬ seq_spec op (abs (M0 !!! T0)) (abs (M0 !!! T0)) vp))) 
-      as [Hcase1 | Hcase2]; clear Hdec.
-    - iMod (inv_alloc (threadN N) _
-              (∃ M T, State γ_sy γ_tk (au N γ_s op Φ) Φ M T op vp T0) 
-                                    with "[AU Hc Hreg_sy1]") as "#HthInv".
-      { iNext. iExists M0, T0. iFrame "Hreg_sy1".
-        iSplitR. { by iPureIntro. }
-        iLeft. unfold Pending. iFrame.
-        unfold past_lin.
-        destruct Hcase1 as [H' | H'].
-        - rewrite H'. iIntros "%Hpast". 
-          destruct Hpast as [t [H'' _]]. lia.
-        - destruct H' as [H1' H2'].
-          rewrite H1'. iIntros "%Hpast". 
-          destruct Hpast as [t [H' Hss]].
-          assert (t = T0) as -> by lia. contradiction. }
-
-      iModIntro. iSplitR "Hproph Token". iNext.
-      iExists M0, T0, s0. iFrame "∗%".
-      iExists (R ∪ {[tid]}), hγt'. iFrame.
-      iSplitR. iPureIntro. subst hγt'.
-      apply leibniz_equiv. rewrite dom_insert.
-      rewrite Domm_hγt. clear; set_solver.
-      rewrite (big_sepS_delete _ (R ∪ {[tid]}) tid); last by set_solver.
-      iSplitR "Hstar_reg". unfold Reg.
-      iExists γ_tk, γ_sy, Φ, op, vp, T0, vtid. iFrame "∗#".
-      assert ((R ∪ {[tid]}) ∖ {[tid]} = R) as H' 
-                  by (clear -tid_notin_R; set_solver).
-      by rewrite H'.
-      
-      iModIntro. wp_bind (dsOp _ _)%E.
-      
-      iAssert (update_helping_protocol N γ_t γ_s γ_td γ_ght)%I as "Upd_help".
-      { admit. }
-      iAssert (thread_vars γ_t γ_ght γ_sy tid T0)%I as "#Thr_vars".
-      { iFrame "#". }
-
-      wp_apply dsOp_spec; try done.
-      iIntros (res)"HpastW".
-      wp_pures.
-      wp_apply ((typed_proph_wp_resolve1 resTTypedProph 
-                  _ _ _ _ _ _ _ (res))
-        with "Hproph"); try done.
-      { unfold typed_proph_from_val; simpl. by rewrite resT_proph_resolve. }  
-      wp_pures. iModIntro. iIntros "%vp_eq_res". subst vp.
-       
-      iApply fupd_wp.
-      
-      iInv "HthInv" as (M1_th T1_th)"(>Hth_sy & >% & Hth_or)".
-      iInv "HInv" as (M1 T1 s1) "(>HCntr & >%Habs1 & >Hist & Help & Templ)".
-      iDestruct "Help" as (R1 hγt1)"(>HR & >Hγt 
-                                  & >Domm_hγt & Hstar_reg)".
-      
-      iAssert (⌜tid ∈ R1⌝)%I as "%".
-      { iPoseProof (own_valid_2 _ _ _ with "[$HR] [$FP_t]") as "H'".
-        iDestruct "H'" as %H'.
-        apply auth_both_valid_discrete in H'.
-        destruct H' as [H' _].
-        apply gset_included in H'.
-        iPureIntro. set_solver. }
-      rename H into tid_in_R1.
-      
-      iAssert (▷ (⌜M1_th = M1⌝ ∗ ⌜T1_th = T1⌝ 
-               ∗ ([∗ set] t_id ∈ R1, Reg N γ_t γ_s γ_ght t_id M1)
-               ∗ own (γ_sy) (to_frac_agree (1 / 2) M1_th) ))%I
-                with "[Hstar_reg Hth_sy]" as "(>% & >% & Hstar_reg & >Hth_sy)". 
-      { 
-        iEval (rewrite (big_sepS_elem_of_acc _ (R1) tid); 
-                                last by eauto) in "Hstar_reg".
-        iDestruct "Hstar_reg" as "(Hreg_t & Hstar_reg')".
-        iDestruct "Hreg_t" as (γ_tk' γ_sy' Q' op' vp' t0' vtid')
-                          "(Hreg_proph & >Hreg_gh' & >Hreg_sy & Ht_reg')".
-
-        iDestruct "Hreg_gh'" as "(Hreg_gh' & #?)".
-        iCombine "Hreg_gh" "Hreg_gh'" as "H".
-        iPoseProof (own_valid with "H") as "Valid".
-        iDestruct "Valid" as %Valid.
-        rewrite auth_frag_valid in Valid.
-        apply singleton_valid in Valid.
-        apply to_agree_op_inv in Valid.
-        apply leibniz_equiv in Valid.
-        injection Valid; intros <- <-.
-                  
-        iAssert (⌜M1_th = M1 ∧ T1_th = T1⌝)%I as "(% & %)".
-        { iPoseProof (own_valid_2 _ _ _ with "[$Hth_sy] [$Hreg_sy]") 
-              as "V_M".
-          iDestruct "V_M" as %V_M.
-          apply frac_agree_op_valid in V_M. destruct V_M as [_ V_M].
-          iPureIntro. split; first by apply leibniz_equiv. admit. } 
-        subst M1_th T1_th.
-          
-        iSplitR. { by iPureIntro. } 
-        iSplitR. iNext; by iPureIntro.
-        iSplitR "Hth_sy". iApply "Hstar_reg'".
-        iNext. iExists γ_tk', γ_sy, Q', op', vp', T0, vtid'.
-        iFrame "∗#". by iNext. 
-      } subst M1_th T1_th.
-      
-      iEval (unfold past_lin_witness) in "HpastW".
-      (* iEval (rewrite Upd_thr) in "HpastW".*)
-
-      iDestruct "Hth_or" as "[Hth_or | Hth_or]".
-      { iDestruct "Hth_or" as "(AU & Hc & >%HPending)".
-        destruct (decide (updater_thread op res = true))
-          as [Hdec | Hdec]. 
-        - rewrite Hdec. rewrite Hdec in HPending.
-          iExFalso. admit. 
-        - destruct (decide (updater_thread op res = false)) as [Hdec' | Hdec'].
-          + rewrite Hdec'. rewrite Hdec' in HPending. 
-            iExFalso. admit.
-          + admit. }  
-      
-      iDestruct "Hth_or" as "(Hth_or & Hpast)".  
-      iDestruct "Hth_or" as "[Hth_or | >Hth_or]"; last first.
-      { iPoseProof (own_valid_2 _ _ _ with "[$Token] [$Hth_or]") as "%".
-        exfalso; try done. }
-        
-      iModIntro. iSplitR "Hth_or Hth_sy Token Hpast".
-      iExists M1, T1, s1; iFrame "∗%".
-      iNext. iExists R1, hγt1; iFrame.     
-
-      iModIntro. iSplitL "Token Hth_sy Hpast".
-      iNext. iExists M1, T1. iFrame "Hth_sy". 
-      iSplitR. by iPureIntro. iRight. iFrame "∗%".
-      by subst T1.
-      
-      iModIntro. by wp_pures.
-    - assert (updater_thread op vp = false 
-        ∧ seq_spec op (abs (M0 !!! T0)) (abs (M0 !!! T0)) vp) as [Upd_thr Hss]. 
-      { clear -Hcase2. destruct (updater_thread op vp); split.
-        - exfalso; apply Hcase2. left; try done.
-        - exfalso; apply Hcase2. left; try done. 
-        - done. 
-        - assert (Decision (seq_spec op (abs (M0 !!! T0)) (abs (M0 !!! T0)) vp)) as H'.
-          { apply seq_spec_dec. }
-          destruct (decide (seq_spec op (abs (M0 !!! T0)) (abs (M0 !!! T0)) vp));
-            try done. 
-          exfalso. apply Hcase2. right.
-          split; try done. } 
-      iMod "AU" as (c) "[Cntr [_ Hcomm]]".
-      iAssert (⌜c = abs s0⌝)%I as "%". { admit. } subst c. 
-      iSpecialize ("Hcomm" $! (abs s0) vp). 
-      iMod ("Hcomm" with "[Cntr]") as "HΦ".
-      { iFrame. rewrite Habs0 in Hss. by iPureIntro. }
-   
-      iAssert (past_lin M0 T0 op vp T0)%I as "Hpast".
-      { iPureIntro. rewrite Upd_thr. exists T0.
-        split; try done. }
-        
-      iMod (inv_alloc (threadN N) _
-            (∃ M T, State γ_sy γ_tk (au N γ_s op Φ) Φ M T op vp T0) 
-                                  with "[Hreg_sy1 Token]") as "#HthInv".
-      { iNext. iExists M0, T0. iFrame "Hreg_sy1".
-        iSplitR. by iPureIntro.
-        iRight. unfold Done. iFrame "Hpast".
-        by iRight. }
-      
-      iAssert (update_helping_protocol N γ_t γ_s γ_td γ_ght)%I as "Upd_help".
-      { admit. }
-      iAssert (thread_vars γ_t γ_ght γ_sy tid T0)%I as "#Thr_vars".
-      { iFrame "#". }
-  
-      
-      iModIntro. iSplitR "Hproph HΦ". iNext.
-      iExists M0, T0, s0.  iFrame "∗%".
-      iExists (R ∪ {[tid]}), hγt'. iFrame.
-      iSplitR. iPureIntro. subst hγt'.
-      apply leibniz_equiv. rewrite dom_insert.
-      rewrite Domm_hγt. clear; set_solver.
-      rewrite (big_sepS_delete _ (R ∪ {[tid]}) tid); last by set_solver.
-      iSplitR "Hstar_reg". unfold Reg.
-      iExists γ_tk, γ_sy, Φ, op, vp, T0, vtid. iFrame "∗#".
-      assert ((R ∪ {[tid]}) ∖ {[tid]} = R) as H' 
-                by (clear -tid_notin_R; set_solver).
-      by rewrite H'.  
-        
-      iModIntro.
-      wp_apply dsOp_spec; try done.
-      iIntros (res)"HpastW". wp_pures.
-      wp_apply ((typed_proph_wp_resolve1 resTTypedProph 
-                  _ _ _ _ _ _ _ (res))
-        with "Hproph"); try done.
-      { unfold typed_proph_from_val; simpl. by rewrite resT_proph_resolve. }    
-      wp_pures. iModIntro. iIntros "->".
-      wp_pures. iModIntro. done. 
-*)
-  Admitted.
-  
-End CLIENT_SPEC.
-
-Module SEARCH_STRUCTURE : ABSTRACT_DATA_TYPE with Definition absTUR := gsetUR nat.
-
-  Parameter search : val.
-  Parameter insert : val.
-  Parameter delete : val.
-
-  Definition dsOp : val :=
-  λ: "OP" "r" "k",     
-    if: "OP" = #0 
-    then search "r" "k"
-    else if: "OP" = #1 
-    then insert "r" "k"
-    else delete "r" "k".
-
-  (* Definition K := Z. *)
-  Inductive Opp := searchOp : nat → Opp | insertOp : nat → Opp | deleteOp : nat → Opp.
-  Definition Op := Opp.
-
-  Definition Op_to_val (op: Op) : val :=
-    match op with
-    | searchOp _ => #0
-    | insertOp _ => #1
-    | deleteOp _ => #2 
-    end.
-    
-  Definition absTUR := gsetUR nat.
-  Definition absT := ucmra_car absTUR.
-
-  Definition resT := bool.
-  Definition resT_to_base_lit (b: resT) : base_lit := LitBool b.
-  Coercion resT_to_base_lit : resT >-> base_lit.
-  Definition resT_from_val (v : val) : option bool :=
-    match v with
-    | LitV(LitBool b) => Some b
-    | _               => None
-    end.
-  Definition resT_to_val (b : bool) : val := LitV(LitBool b).
-  
-  Lemma resT_inj_prop : ∀ (b : bool), bool_from_val (bool_to_val b) = Some b.
-  Proof. done. Qed.
-
-  Definition resTProph : TypedProphSpec :=
-    mkTypedProphSpec resT resT_from_val resT_to_val resT_inj_prop.
-  Definition resTTypedProph `{!heapGS Σ} := make_TypedProph resTProph.
-
-  Lemma resT_proph_resolve : ∀ (res: resT), resT_from_val #res = Some res.
-  Proof. try done. Qed.
-
-  Definition seq_spec (op: Op) (C: absT) (C': absT) (res: bool) : Prop :=
-    match op with
-    | searchOp k => C' = C ∧ (if res then k ∈ C else k ∉ C)
-    | insertOp k => C' = C ∪ {[k]} ∧ (if res then k ∉ C else k ∈ C)
-    | deleteOp k => C' = C ∖ {[k]} ∧ (if res then k ∈ C else k ∉ C)
-    end.
-
-  Global Instance seq_spec_dec : ∀ op c c' res, Decision (seq_spec op c c' res).
-  Proof.
-    intros op c c' res. unfold seq_spec. 
-    destruct op; try apply and_dec; try destruct res; try apply _.
-  Qed.
-
-  Definition updater_thread (op: Op) (res: resT) : bool := 
-    match op, res with
-    | searchOp _, _ => false
-    | _, false => false
-    | _, _ => true
-    end.
-
-  Global Instance updater_thread_dec: ∀ op res b, 
-    Decision (updater_thread op res = b).
-  Proof.
-    intros op res b. unfold updater_thread.
-    destruct op; destruct res; try apply _.
-  Qed.  
-
-  Global Instance Op_inhabited : Inhabited Op := populate (searchOp 0).
-  Global Instance absTUR_discrete : CmraDiscrete absTUR.
-  Proof. try apply _. Qed.
-  Global Instance resT_inhabited : Inhabited resT.
-  Proof. try apply _. Qed.
-
-End SEARCH_STRUCTURE.
-
-Module SKIPLIST0 <: DATA_STRUCTURE SEARCH_STRUCTURE.
-  Import SEARCH_STRUCTURE.
-  
-  (*
-    The snapshot stores:
-    0) set of nodes
-    1) ghost location for interface
-    2) global interface
-    3) ghost location for keyset
-    4) global contents
-    5) map from nodes to node-local info
-
-    Node local info:
-    1) singleton interface
-    2) keyset
-    3) physical contents
-    4) Marking
-  *)
-
-  
-  Definition snapshotUR := natUR.
-  Definition snapshot := ucmra_car snapshotUR.
-  
-  Definition abs (s: snapshot) : absT := ∅.
-
-  Global Instance snapshotUR_discrete : CmraDiscrete snapshotUR.
-  Proof. try apply _. Qed.
-
-  Global Instance snapshot_leibnizequiv : LeibnizEquiv (snapshot).
-  Proof. try apply _. Qed.
-  
-  Global Instance snapshot_inhabited : Inhabited snapshot := populate 0.
-  
-  Parameter inContents : val.
-  Parameter findNext : val.
-  Parameter try_constraint : val.
-  Parameter maintenance : val.
-  Parameter createNode: val.
-
-  (** Template algorithms *)
-
-  Definition traverse_rec (r: Node) : val :=
-    rec: "tr" "p" "c" "k" :=
-      let: "fn_ck" := findNext "c" "k" in
-      if: Fst "fn_ck" then
-        match: Snd "fn_ck" with
-          NONE => ""
-        | SOME "s" =>
-            match: try_constraint "p" "c" "s" with
-              NONE =>
-                let: "fn_hk" := findNext #r "k" in
-                match: Snd "fn_hk" with
-                  NONE => ""
-                | SOME "n" => 
-                    "tr" #r "n" "k" end
-            | SOME "_" => "tr" "p" "s" "k" end end  
-      else
-        match: Snd "fn_ck" with
-          NONE => ("p", "c")
-        | SOME "s" => "tr" "c" "s" "k" end.
-
-  Definition traverse (r: Node) : val := 
-    λ: "k", 
-      let: "fn_hk" := findNext #r "k" in
-      match: Snd "fn_hk" with
-        NONE => ""
-      | SOME "n" => 
-          traverse_rec r #r "n" "k" end.
-
-  Definition search (r: Node) : val :=
-    λ: "k",
-      let: "pc" := traverse r "k" in
-      let: "c" := Snd "pc" in
-      inContents "c" "k".
-      
-  Definition delete (r: Node) : val :=
-    λ: "k",
-      let: "pc" := traverse r "k" in
-      let: "c" := Snd "pc" in
-      if: ~ (inContents "c" "k") then
-        #false
-      else
-        match: try_constraint "c" with
-          NONE => #false
-        | SOME "_" => maintenance "k";; #true end.
-        
-  Definition insert (r: Node) : val :=
-    rec: "ins" "k" :=
-      let: "pc" := traverse r "k" in
-      let: "p" := Fst "pc" in
-      let: "c" := Snd "pc" in
-      if: inContents "c" "k" then
-        #false
-      else
-        let: "e" := createNode "k" "c" in
-        match: try_constraint "p" "c" "e" with
-          NONE => "ins" "k"
-        | SOME "_" => #true end.
-  
-  Definition esT : Type := gmap Node (gset nat).
-
-  Definition flowUR := authR (multiset_flowint_ur nat).
-  Definition auth_keysetUR := authUR $ (keysetUR nat).
-  Definition auth_setnodeUR := authUR $ (gsetUR Node).
-
-  Class skG Σ := SK {
-                    sk_flowG :> inG Σ flowUR;
-                    sk_auth_keysetG :> inG Σ auth_keysetUR;
-                    sk_auth_setnodeG :> inG Σ auth_setnodeUR;
-                   }.
-                 
-  Definition skΣ : gFunctors :=
-    #[ GFunctor flowUR;  GFunctor auth_keysetUR;
-       GFunctor auth_setnodeUR ].
-  
-  Instance subG_skΣ {Σ} : subG skΣ Σ → skG Σ.
-  Proof. solve_inG. Qed.
-
-  Section skiplist_v0.
-    Context {Σ} `{!heapGS Σ, !skG Σ}.
-    Notation iProp := (iProp Σ).
-  
-    Parameter node : Node → bool → esT → (gset nat) → iProp.
-    Parameter node_timeless_proof : ∀ r n es V, Timeless (node r n es V).
-    Global Instance node_timeless r n es V: Timeless (node r n es V).
-    Proof. apply node_timeless_proof. Qed.  
-
-    Parameter Mark : snapshot → Node → bool.
-    Parameter ES : snapshot → Node → esT.
-    Parameter PC : snapshot → Node → gset nat.
-    Parameter GFI : snapshot → (multiset_flowint_ur nat).
-    Parameter FI : snapshot → Node → (multiset_flowint_ur nat).
-    Parameter FP : snapshot → gset Node.
-  
-    Definition Cont (s: snapshot) (n: Node) : gset nat :=
-      if decide (Mark s n) then ∅ else PC s n.
-
-    Parameter out_set : multiset_flowint_ur nat → gset nat.
-    (* out_es es := ⋃_n es !!! n *)
-    Parameter out_es : esT → gset nat.
-    Parameter keyset : multiset_flowint_ur nat → gset nat. 
-    
-    (** data structure specific inv *)
-
-    Definition globalRes γ_I γ_fp γ_ks s : iProp :=
-        own γ_I (● (GFI s)) 
-      ∗ own γ_fp (● FP s) 
-      ∗ own γ_ks (● prod (KS, abs s)).
-    
-    Definition outflow_constraint (In: multiset_flowint_ur nat) (esn: esT) : Prop := True.
-  
-    Definition node_inv_pure s n : iProp :=
-        ⌜¬ (Mark s n) → out_set (FI s n) ⊆ inset nat (FI s n) n⌝
-      ∗ ⌜Cont s n ⊆ keyset (FI s n)⌝
-      ∗ ⌜Mark s n → out_set (FI s n) ≠ ∅⌝
-      ∗ ⌜outflow_constraint (FI s n) (ES s n)⌝ .
-
-    Definition node_inv γ_I γ_ks s n : iProp :=
-        node n (Mark s n) (ES s n) (PC s n)
-      ∗ own γ_I (◯ (FI s n))
-      ∗ own γ_ks (◯ prod (keyset (FI s n), Cont s n))
-      ∗ node_inv_pure s n.   
-
-    Definition per_tick_inv r s : iProp := 
-        ⌜inset nat (FI s r) r = KS⌝ ∗ ⌜out_set (FI s r) = KS⌝
-      ∗ ⌜¬ Mark s r⌝
-      ∗ [∗ set] n ∈ (FP s), node_inv_pure s n.
-    
-    Definition transition_inv s s' : Prop :=
-        (∀ n, n ∈ FP s → Mark s n → ES s' n = ES s n)
-      ∧ (∀ n, n ∈ FP s → Mark s n → Mark s' n)
-      ∧ (∀ n, n ∈ FP s → ¬ Mark s n → Mark s' n → ES s n ≠ ES s' n)
-      ∧ (∀ n, n ∈ FP s → PC s n = PC s' n)
-      ∧ (FP s ⊆ FP s').
-
-    Definition skiplist_inv γ_I γ_fp γ_ks r (M: gmap nat snapshot) 
-      (T: nat) (s: snapshot) : iProp :=
-        globalRes γ_I γ_fp γ_ks s
-      ∗ ([∗ set] n ∈ FP s, node_inv γ_I γ_ks s n)
-      ∗ ([∗ set] t ∈ dom M, per_tick_inv r (M !!! t))
-      ∗ ⌜∀ t, 0 ≤ t < T → transition_inv (M !!! t) (M !!! (t+1)%nat)⌝
-      ∗ ⌜transition_inv (M !!! T) s⌝.
-    
-    Instance skiplist_inv_timeless γ_I γ_fp γ_ks r M T s : 
-      Timeless (skiplist_inv γ_I γ_fp γ_ks r M T s).
-    Proof.
-    Admitted.  
-
-    (** Helper functions specs *)
-    
-    Parameter inContents_spec : ∀ (k: nat) (n: Node),
-       ⊢ (<<< ∀∀ m es pc, node n m es pc >>>
-             inContents #n #k @ ⊤
-         <<< ∃∃ (v: bool),
-                node n m es pc ∗ ⌜v ↔ k ∈ pc⌝,
-                RET #v >>>)%I.
-
-    Parameter findNext_spec : ∀ (k: nat) (n: Node),
-       ⊢ (<<< ∀∀ m es pc, node n m es pc >>>
-             findNext #n #k @ ⊤
-         <<< ∃∃ (success: bool) (n': Node),
-                node n m es pc
-              ∗ (match success with true => ⌜k ∈ es !!! n'⌝ 
-                                  | false => ⌜k ∉ out_es es⌝ end),
-             RET (match success with true => (#m, SOMEV #n') 
-                                   | false => (#m, NONEV) end)  >>>)%I.
-                                 
-    Definition edgset_update es k curr succ : esT :=
-      <[ succ := (es !!! succ) ∪ {[k]} ]>
-        (<[ curr := (es !!! curr) ∖ {[k]} ]> es).
-
-    Parameter try_constraint_trav_spec : ∀ (k: nat) (pred curr succ: Node),
-       ⊢ (<<< ∀∀ m es pc, node pred m es pc >>>
-             try_constraint #pred #curr #succ @ ⊤
-         <<< ∃∃ (success: bool) es',
-                node pred m es' pc
-              ∗ (match success with true => ⌜m = false⌝ ∗ ⌜k ∈ es !!! curr⌝
-                                            ∗ ⌜es' = edgset_update es k curr succ⌝ 
-                                  | false => ⌜m = true ∨ k ∉ es !!! curr⌝
-                                             ∗ ⌜es' = es⌝ end),
-                RET (match success with true => SOMEV #() 
-                                      | false => NONEV end)  >>>)%I.
-  
-    Parameter createNode_spec : ∀ (k: nat) (n: Node),
-       ⊢ ({{{ True }}}
-             createNode #k #n
-         {{{ e m es pc, RET #e;
-                node e m es pc
-              ∗ ⌜k ∈ pc⌝
-              ∗ ⌜k ∈ es !!! n⌝ }}})%I.
-  
-    Parameter try_constraint_insert_spec : ∀ (k: nat) (pred curr entry: Node),
-       ⊢ (<<< ∀∀ m es pc, node pred m es pc >>>
-             try_constraint #pred #curr #entry @ ⊤
-         <<< ∃∃ (success: bool) es',
-                node pred m es' pc
-              ∗ (match success with true => ⌜m = false⌝ ∗ ⌜k ∈ es !!! curr⌝
-                                            ∗ ⌜es' = edgset_update es k curr entry⌝ 
-                                  | false => ⌜m = true ∨ k ∉ es !!! curr⌝
-                                             ∗ ⌜es' = es⌝ end),
-                RET (match success with true => SOMEV #() 
-                                      | false => NONEV end)  >>>)%I.
-End skiplist_v0.   
-    
-End SKIPLIST0.
-
-Module SKIPLIST_SPEC : HINDSIGHT_SPEC SEARCH_STRUCTURE SKIPLIST0.
-  Module DEFS := HINDSIGHT_DEFS SEARCH_STRUCTURE SKIPLIST0.
-  Import SEARCH_STRUCTURE SKIPLIST0 DEFS.
-  
-  Context {Σ} `{!heapGS Σ, !skG DEFS.Σ}.
-  Notation iProp := (iProp Σ).
-  Context {γ_I γ_fp γ_ks: gname}.
-
-  Lemma dsOp_spec: ∀ N γ_s γ_t γ_m γ_td γ_ght op r (template_inv := skiplist_inv γ_I γ_fp γ_ks r) γ_sy t_id t0,
-          ds_inv N γ_t γ_s γ_m γ_td γ_ght (skiplist_inv γ_I γ_fp γ_ks r) -∗
-            □ update_helping_protocol N γ_t γ_s γ_td γ_ght -∗
-              thread_vars γ_t γ_ght γ_sy t_id t0 -∗
-                {{{ True }}} 
-                     dsOp (Op_to_val op) #r
-                {{{ res, RET #res; past_lin_witness γ_m op res t0  }}}.
-  Proof.
-  Admitted.              
-                
-                
-
-End SKIPLIST_SPEC.
