templates/lockfree/skiplist_v0_search.v
@@ -11,30 +11,58 @@ From iris.heap_lang.lib Require Import nondet_bool.
 From iris.bi.lib Require Import fractional.
 Set Default Proof Using "All".
 From iris.bi.lib Require Import fractional.
-Require Export skiplist_v0_traverse.
+Require Export skiplist_v0.
 
-Section skiplist_v0_search.
+Module SKIPLIST0_SPEC_SEARCH.
+  Module DEFS := HINDSIGHT_DEFS SKIPLIST0.
+  Import DEFS SKIPLIST0.
 
-  Context {Σ} `{!heapGS Σ, !dsG Σ, !skG Σ}.
-  Notation iProp := (iProp Σ).
+  Parameter inContents_spec : ∀ (k: nat) (n: Node),
+     ⊢ (<<< ∀∀ m es pc, node n m es pc >>>
+           inContents #n #k @ ⊤
+       <<< ∃∃ (v: bool),
+              node n m es pc ∗ ⌜v ↔ k ∈ pc⌝,
+              RET #v >>>)%I.
 
+
+  Lemma traverse_spec N γ_t γ_s γ_m γ_td γ_ght r γ_sy t_id t0 
+    (k: nat) :
+    ⌜k ∈ KS⌝ -∗
+      main_inv N γ_t γ_s γ_m γ_td γ_ght -∗
+       thread_vars γ_t γ_ght γ_sy t_id t0 -∗  
+        {{{ True }}}
+           traverse r #k
+        {{{ (p c: Node) s, RET (#p, #c); 
+              past_state γ_m t0 s
+            ∗ ⌜p ∈ FP s⌝ ∗ ⌜c ∈ FP s⌝   
+            ∗ ⌜¬ Mark s p⌝
+            ∗ ⌜k ∈ inset nat (FI s p) p⌝
+            ∗ ⌜k ∈ outset nat (FI s p) c⌝
+            ∗ ⌜¬ Mark s c⌝
+            ∗ ⌜k ∈ keyset (FI s c)⌝ }}}.
+  Proof.
+  Admitted.
   
-  Lemma searchOp_spec N γ_s γ_t γ_m γ_td γ_ght γ_I γ_fp γ_ks r (k: K) γ_sy t_id t0:
-        ⌜k ∈ KS⌝ -∗
-          css_inv N γ_t γ_s γ_m γ_td γ_ght (skiplist_inv γ_I γ_fp γ_ks r) -∗
+  Lemma searchOp_spec: ∀ N γ_s γ_t γ_m γ_td γ_ght (r: Node) 
+                      γ_sy t_id t0 (k: nat),
+          main_inv N γ_t γ_s γ_m γ_td γ_ght -∗
             □ update_helping_protocol N γ_t γ_s γ_td γ_ght -∗
               thread_vars γ_t γ_ght γ_sy t_id t0 -∗
                 {{{ True }}} 
-                     search r #k
-                {{{ res, RET #res; past_lin_witness γ_m searchOp k res t0  }}}.
+                     search #r #k
+                {{{ res, RET #res; 
+                      past_lin_witness γ_m (searchOp k) res t0 }}}.
   Proof.
-    iIntros "%k_in_KS #HInv #HUpd #Thd". iIntros (Φ) "!# _ Hpost".
+    iIntros (N γ_s γ_t γ_m γ_td γ_ght r γ_sy t_id t0 k)"#HInv #HUpd #Thd". 
+    iIntros (Φ) "!# _ Hpost".
+    assert (k ∈ KS) as k_in_KS.
+    { admit. }
     wp_lam. wp_pures.
     wp_apply traverse_spec; try done.
     iIntros (p c s) "(#Hpast & %)".
     destruct H as [FP_p [FP_c [Unmarked_p [k_in_ins_p 
       [k_in_outs_p [Unmarked_c k_in_ks_c]]]]]].
-    wp_pures.
+    wp_pures. Locate inContents_spec.
     awp_apply (inContents_spec); try done.
     iInv "HInv" as (M0 T0 s0) "(>CSS & >%Habs0 & >Hist & Help & >Templ)".
     { admit. }
@@ -57,14 +85,16 @@ Section skiplist_v0_search.
     iAssert (⌜t ∈ dom M0⌝)%I as %t_in_M0.
     { admit. }
     apply PT0 in t_in_M0.
-    iAssert (⌜M0 !!! t = s⌝)%I as %M0_t_s.
-    { admit. } rewrite M0_t_s in t_in_M0. 
-    destruct t_in_M0 as [Ins_r [Out_r [Mark_r Hbig_star]]].
+    iAssert (⌜M0 !!! t ≡ s⌝)%I as %M0_t_s.
+    { admit. } 
+    assert (per_tick_inv skiplist_v0.SKIPLIST0.r s) as t_in_M0'.
+    { admit. } 
+    destruct t_in_M0' as [Ins_r [Out_r [Mark_r Hbig_star]]].
     pose proof Hbig_star c FP_c as H'.
     assert (PC s c = PC s0 c) as PC_c.
     { admit. }
 
-    iAssert (⌜seq_spec searchOp (Cont s c) (Cont s c) res k⌝)%I as %Seq_spec_c.
+    iAssert (⌜seq_spec (searchOp k) (Cont s c) (Cont s c) res⌝)%I as %Seq_spec_c.
     { iPureIntro. 
       unfold seq_spec. split; try done. destruct res; 
       unfold Cont; destruct (decide (Mark s c)); try done; rewrite PC_c.
@@ -72,7 +102,7 @@ Section skiplist_v0_search.
       - intros ?. by apply Hres. }
     iAssert (⌜Cont s c ⊆ keyset (FI s c)⌝)%I as %cc_sub_ksc.
     { iPureIntro. by destruct H' as [? [? _]]. }
-    iAssert (⌜seq_spec searchOp (abs s) (abs s) res k⌝)%I as %Seq_spec.
+    iAssert (⌜seq_spec (searchOp k) (abs s) (abs s) res⌝)%I as %Seq_spec.
     { iPureIntro. unfold seq_spec. split; try done. destruct res.
       - assert (k ∈ Cont s c) as H''.
         { unfold Cont. rewrite decide_False; try done.
@@ -85,7 +115,7 @@ Section skiplist_v0_search.
         assert (∀ s n k, k ∈ keyset (FI s n) → (k ∈ (Cont s n) ↔ k ∈ abs s)).
         { admit. }
         admit. }
-    iAssert (past_lin_witness γ_m searchOp k res t0) as "Witn".
+    iAssert (past_lin_witness γ_m (searchOp k) res t0) as "Witn".
     { unfold past_lin_witness, updater_thread. iExists s.
       iFrame "#". by iPureIntro. }
 
@@ -95,6 +125,6 @@ Section skiplist_v0_search.
       iFrame "∗%".
       rewrite (big_sepS_delete _ (FP s0) c); last by eauto.
       iFrame "Res_rest". iFrame. }
-  Admitted.      
-    
-End skiplist_v0_search.
+  Admitted.
+
+End SKIPLIST0_SPEC_SEARCH.
