templates/lockfree/skiplist_v0_spec.v
@@ -1,0 +1,73 @@
+From iris.algebra Require Import excl auth cmra gmap agree gset numbers.
+From iris.algebra.lib Require Import dfrac_agree.
+From iris.heap_lang Require Export notation locations lang.
+From iris.base_logic.lib Require Export invariants.
+From iris.program_logic Require Export atomic.
+From iris.proofmode Require Import tactics.
+From iris.heap_lang Require Import proofmode par.
+From iris.heap_lang.lib Require Import nondet_bool.
+From iris.bi.lib Require Import fractional.
+Set Default Proof Using "All".
+From iris.bi.lib Require Import fractional.
+Require Export skiplist_v0 hindsight_proof.
+
+
+Module SKIPLIST_SPEC : HINDSIGHT_SPEC SKIPLIST0.
+  Module DEFS := HINDSIGHT_DEFS SKIPLIST0.
+  Import SKIPLIST0.
+  
+  Lemma searchOp_spec: ∀ N γ_s γ_t γ_m γ_td γ_ght (r: Node) 
+                      γ_sy t_id t0 (k: nat),
+          DEFS.main_inv N γ_t γ_s γ_m γ_td γ_ght -∗
+            □ DEFS.update_helping_protocol N γ_t γ_s γ_td γ_ght -∗
+              DEFS.thread_vars γ_t γ_ght γ_sy t_id t0 -∗
+                {{{ True }}} 
+                     search #r #k
+                {{{ res, RET #res; 
+                    DEFS.past_lin_witness γ_m (searchOp k) res t0 }}}.
+  Proof.
+  Admitted.
+
+  Lemma insertOp_spec: ∀ N γ_s γ_t γ_m γ_td γ_ght (r: Node) 
+                      γ_sy t_id t0 (k: nat),
+          DEFS.main_inv N γ_t γ_s γ_m γ_td γ_ght -∗
+            □ DEFS.update_helping_protocol N γ_t γ_s γ_td γ_ght -∗
+              DEFS.thread_vars γ_t γ_ght γ_sy t_id t0 -∗
+                {{{ True }}} 
+                     insert #r #k
+                {{{ res, RET #res; 
+                    DEFS.past_lin_witness γ_m (insertOp k) res t0 }}}.
+  Proof.
+  Admitted.
+
+  Lemma deleteOp_spec: ∀ N γ_s γ_t γ_m γ_td γ_ght (r: Node) 
+                      γ_sy t_id t0 (k: nat),
+          DEFS.main_inv N γ_t γ_s γ_m γ_td γ_ght -∗
+            □ DEFS.update_helping_protocol N γ_t γ_s γ_td γ_ght -∗
+              DEFS.thread_vars γ_t γ_ght γ_sy t_id t0 -∗
+                {{{ True }}} 
+                     delete #r #k
+                {{{ res, RET #res; 
+                    DEFS.past_lin_witness γ_m (deleteOp k) res t0 }}}.
+  Proof.
+  Admitted.
+
+  
+  Lemma dsOp_spec: ∀ N γ_s γ_t γ_m γ_td γ_ght op (r: Node) 
+                      γ_sy t_id t0,
+          DEFS.main_inv N γ_t γ_s γ_m γ_td γ_ght -∗
+            □ DEFS.update_helping_protocol N γ_t γ_s γ_td γ_ght -∗
+              DEFS.thread_vars γ_t γ_ght γ_sy t_id t0 -∗
+                {{{ True }}} 
+                     dsOp (Op_to_val op) #r
+                {{{ res, RET #res; DEFS.past_lin_witness γ_m op res t0 }}}.
+  Proof.
+    iIntros (N γ_s γ_t γ_m γ_td γ_ght op r γ_sy t_id t0) "#HInv #HUpd #Thd_vars".
+    unfold dsOp. iIntros (Φ) "!# _ Hpost". wp_lam. wp_pure.
+    unfold Op_to_val; destruct op as [k|k|k].
+    - wp_pures. wp_apply searchOp_spec; try done.
+    - wp_pures. wp_apply insertOp_spec; try done.
+    - wp_pures. wp_apply deleteOp_spec; try done.
+  Qed.
+
+End SKIPLIST_SPEC. 
